

1

$$G(x) = \int_a^x f(u) (x-u) du = x \int_a^x f(u) du - \int_a^x f(u) u du$$

$$G'(x) = x f(x) + \int_a^x f(u) du - f(x) x \quad (\text{By the fund. theorem of calc.})$$

$$= \int_a^x f(u) du$$

let $x=u$, $u=t$

$$G'(u) = \int_a^u f(t) dt, \text{ For } G'(u) \text{ is continuous,}$$

$$\Rightarrow \int_a^x \int_a^u f(t) dt du = \int_a^x G'(u) du$$

$$= G(x) - G(a) \quad (\text{By the fund. theorem of calc.})$$

$$\text{With } G(a) = \int_a^a f(u) (x-u) du = 0$$

Hence

$$\int_a^x \int_a^u f(t) dt du = G(x) = \int_a^x f(u) (x-u) du$$

2 i) • For even n , $n=2k$, $k \in \mathbb{N}$

let $\epsilon > 0$

$$\begin{aligned} |x^n e^x - 0| &= |x^n| e^x && \text{(absolute law)} \\ &= x^n e^x && \text{(for } x^{2k} \geq 0 \\ &= \frac{x^n}{e^{-x}} && \text{e}^x > 0 \end{aligned}$$

From lectures, we know that $\lim_{x \rightarrow \infty} \frac{e^x}{x^n} = \infty$ (*) for $x > 1$
 $\Rightarrow \lim_{x \rightarrow -\infty} \frac{e^{-x}}{(-x)^n} = \infty$, for $x < -1$

But n is even, $(-x)^n = x^n$

so let $N = \frac{1}{\epsilon}$

$$\exists a < -1, \forall x < a \Rightarrow \frac{e^{-x}}{x^n} > N = \frac{1}{\epsilon} \quad (\text{for } (*))$$

$$\Rightarrow \frac{x^n}{e^{-x}} < \epsilon \quad (\text{Ineq. law})$$

Hence $\lim_{x \rightarrow -\infty} x^n e^x = 0$ for even n

• If n is odd, $n=2k-1$, for $k \in \mathbb{N}$

$$\begin{aligned} \lim_{x \rightarrow -\infty} x^n e^x &= \lim_{x \rightarrow -\infty} x^{2k} e^x x^{-1} && \text{(exponential law)} \\ &= \lim_{x \rightarrow -\infty} e^{2k} e^x \lim_{x \rightarrow -\infty} \frac{1}{x} && \text{(limit product)} \\ &= 0 \times 0 \\ &= 0 \end{aligned}$$

Tianmu, Qi 1473217

2 ii) suppose $p_n(x) = ax^n + p_{n-1}(x)$, $a \neq 0$

$$(*) \lim_{x \rightarrow \infty} p_n(x) = a \lim_{x \rightarrow \infty} x^n + p_{n-1}(x) \\ = a \times \infty \quad (\text{from lecture})$$

$$= \begin{cases} \infty & \text{if } a > 0 \\ -\infty & \text{if } a < 0 \end{cases}$$

• If $a < 0$,

let $N > 0$, because $\lim_{x \rightarrow \infty} \frac{e^x}{x} = \infty$ (by lemma)

$$\exists k_1 > 1, \forall x > k_1$$

$$\Rightarrow \frac{e^x}{x} > N$$

And as $\lim_{x \rightarrow \infty} p_n(x) = \infty$, by (*)

$$\exists k_2 > 0, \forall x > k_2$$

$$\Rightarrow p_n(x) > k_1 \Rightarrow \frac{e^{p_n(x)}}{p_n(x)} > N$$

Here $\forall x > k_2 > 0$

$$\Rightarrow \frac{e^{p_n(x)}}{p_n(x)} > N,$$

$$\Rightarrow \lim_{x \rightarrow \infty} \frac{e^{p_n(x)}}{p_n(x)} = \infty \quad \text{when } a > 0$$

2) ii) continued.

• if $a < 0$

Notice that

$$\lim_{x \rightarrow \infty} \frac{e^x}{-x} = \lim_{x \rightarrow \infty} \frac{-1}{xe^x} = 0 \quad \left(\text{for } \lim_{x \rightarrow \infty} xe^x = \infty \text{ from lecture} \right)$$

Here let $q_n(x) = -p_n(x)$ thus $\lim_{x \rightarrow \infty} q_n(x) = -\lim_{x \rightarrow \infty} p_n(x) = \infty$, by (*)

$$\lim_{x \rightarrow \infty} \frac{e^{p_n(x)}}{p_n(x)} = \lim_{x \rightarrow \infty} \frac{e^{-q_n(x)}}{-q_n(x)}$$

$$= \lim_{x \rightarrow k} \frac{e^{-x}}{-x}$$

$$= 0$$

(where $k = \lim_{x \rightarrow \infty} q_n(x) = \infty$
using the continuous comp. theorem)

• Hence, if $p_n(x) = ax^n + \dots$

$$\lim_{x \rightarrow \infty} \frac{\exp(p_n(x))}{p_n(x)} = \begin{cases} \infty & \text{if } a > 0 \\ 0 & \text{if } a < 0 \end{cases}$$

3 i) let $N > 0$, define $f(a) = g(a) = 0$

• for $\lim_{x \rightarrow a} \frac{f'(x)}{g'(x)} = \infty$,

$$\exists \delta > 0 \quad \forall x, 0 < |x - a| < \delta$$

$$\Rightarrow \frac{f'(x)}{g'(x)} > N \Rightarrow g'(x) \neq 0. \quad \text{imply that } f'(a) \text{ and } g'(a) \text{ are continuous in } (a - \delta, a + \delta)$$

• for $\lim_{x \rightarrow a} f(x) = \lim_{x \rightarrow a} g(x) = 0$, take $\epsilon = 1$

$$\exists \delta_2, \delta_3 > 0, \text{ where } \forall x, |x - a| < \min(\delta_2, \delta_3) = 2\delta$$

$$\text{where } |f(x)| < \epsilon, |g(x)| < \epsilon$$

imply that $f(x), g(x)$ are continuous in $[a - \delta, a + \delta]$

• Take $d = \min\{\delta, \delta_2\}$

$$\forall x, 0 < |x - a| < d$$

$$\left\{ \begin{array}{l} g(x) - g(a) = g(x) \neq 0 \\ \text{and} \\ g'(a) \neq 0 \\ \text{as the same reason as lecture notes} \end{array} \right\}$$

$$\Rightarrow \frac{f(x)}{g(x)} = \frac{f(x) - f(a)}{g(x) - g(a)}$$

$$= \exists \alpha \in (a, x) \quad \frac{f'(\alpha)}{g'(\alpha)}$$

(for we've defined $f(a) = g(a) = 0$ for continuity)

(By Cauchy's mean value theorem and $f(x), g(x), f'(x), g'(x)$ continuity within $[a, a + d]$)

$$\text{But } |\alpha - a| < d < \delta$$

$$\Rightarrow \frac{f'(\alpha)}{g'(\alpha)} > N$$

$$\Rightarrow \frac{f(x)}{g(x)} > N \quad (\forall x, 0 < |x - a| < d)$$

$$\text{Hence } \lim_{x \rightarrow a} \frac{f(x)}{g(x)} = \infty$$

Tianhui Qi 1473217

$$3 \text{ ii) } f(x) = x, \quad \lim_{x \rightarrow 0} f(x) = 0, \quad a = 0 \\ g(x) = x^3, \quad \lim_{x \rightarrow 0} g(x) = 0$$

$$\text{And, } \lim_{x \rightarrow 0} \frac{f'(x)}{g'(x)} = \lim_{x \rightarrow 0} \frac{1}{3x^2} = \infty$$

$$\text{Hence } \lim_{x \rightarrow 0} \frac{f(x)}{g(x)} = \lim_{x \rightarrow 0} \frac{x}{x^3} = \lim_{x \rightarrow 0} \frac{1}{x^2} = \infty$$

4.

i) $y'' = -v^2 y$

As $f'' = -Av^2 \cos(vt + \theta) = -v^2 f$

ii) suppose y is a potential solution, $v \neq 0$

Consider

$$g = y - y(0) \cos(vt) - \frac{y'(0)}{v} \sin(vt)$$

Notice that

$$g(0) = 0, \quad g'(0) = 0$$

And g is also a solution, for

$$\begin{aligned} g'' &= y'' + y(0)v^2 \cos(vt) + y'(0)v \sin(vt) \\ &= -v^2 y - (-v^2) \left[y(0) \cos(vt) + \frac{y'(0)}{v} \sin(vt) \right] = -v^2 g \end{aligned}$$

consider

$$E = v^2 g^2 + (g')^2$$

$$\begin{aligned} \partial_t E &= 2v^2 g g' + 2g' g'' \\ &= 2g' (v^2 g + g'') \\ &= 0 \end{aligned}$$

Hence by the mean value theorem

for some c , $E = c = (vg)^2 + (g')^2$, But $E(0) = (vg(0))^2 + (g'(0))^2$
 $\Rightarrow c = 0$

Therefore, $vg(t) = 0$, as $v \neq 0$

$$\Rightarrow g(t) = 0, \quad \forall t, \quad \text{thus } y = y(0) \cos(vt) + \frac{y'(0)}{v} \sin(vt)$$

$$a = y(0), \quad b = y'(0)/v$$

Tianmi Qi 1473217

$$4 \text{ (ii)} \cdot a = y(0) = A \cos(\theta)$$

$$b = \frac{y'(0)}{v} = -A v \sin(vt + \theta) / v$$
$$= -A \sin(\theta)$$

• VICE VERSA

v does not depend on a, b

$$a^2 + b^2 = A^2 \cos^2 \theta + A^2 \sin^2 \theta$$
$$= A^2 \quad (\text{as } \sin^2 \theta + \cos^2 \theta = 1)$$

$$\Rightarrow A = \pm \sqrt{a^2 + b^2}$$

For either $A = \sqrt{a^2 + b^2}$ or $-\sqrt{a^2 + b^2}$

$\Rightarrow \theta$ is the solution of both

$$\begin{cases} \cos(\theta) = \frac{a}{A} = \frac{a}{\pm \sqrt{a^2 + b^2}} \\ \sin(\theta) = -\frac{b}{A} = \frac{-b}{\pm \sqrt{a^2 + b^2}} \end{cases}$$

which is unique

$$\text{i.e. } \theta = \arccos\left(\frac{a}{\sqrt{a^2 + b^2}}\right) = \operatorname{arcsin}\left(\frac{-b}{\sqrt{a^2 + b^2}}\right)$$

when the RHS agrees.

Tianrui Qi 1473217

5 i) • As $\lim_{x \rightarrow 0} \ln(1+x) - x + \frac{x^2}{2} - \frac{x^3}{3} = 0$

and $\lim_{x \rightarrow 0} x^3 = 0$

use l'Hôpital's rule

$$l = \lim_{x \rightarrow 0} \frac{\ln(1+x) - x + \frac{x^2}{2} - \frac{x^3}{3}}{x^3}$$

$$= \lim_{x \rightarrow 0} \frac{\frac{1}{1+x} - 1 + x - x^2}{3x^2} \quad \left(\text{for } \frac{d}{dx} \ln(1+x) = \frac{1}{1+x} \right)$$

• Again, $\lim_{x \rightarrow 0} \frac{1}{1+x} - 1 + x - x^2 = 0$

$$\lim_{x \rightarrow 0} 3x^2 = 0$$

use l'Hôpital's rule

$$l = \lim_{x \rightarrow 0} \frac{-\frac{1}{(1+x)^2} + 1 - 2x}{6x}$$

• Again, $\lim_{x \rightarrow 0} -\frac{1}{(1+x)^2} + 1 - 2x = 0$

$$\lim_{x \rightarrow 0} 6x = 0$$

use l'Hôpital's rule

$$l = \lim_{x \rightarrow 0} \frac{\frac{2}{(1+x)^3} - 2}{6} = \frac{2-2}{6} = 0$$

Tianhui Qi 1473247

$$5 \text{ ii) } l = \lim_{x \rightarrow \infty} x \ln \left(1 + \frac{1}{x} \right)$$

$$= \lim_{x \rightarrow \infty} \frac{\ln \left(1 + \frac{1}{x} \right)}{x^{-1}}$$

$$\text{For } \lim_{x \rightarrow \infty} \ln \left(1 + \frac{1}{x} \right) = 0$$

$$\lim_{x \rightarrow \infty} \frac{1}{x} = 0$$

• Apply L'Hôpital's rule

$$l = \lim_{x \rightarrow \infty} \frac{1}{1 + \frac{1}{x}} \times \frac{-\frac{1}{x^2}}{-\frac{1}{x^2}}$$

$$= \lim_{x \rightarrow \infty} \frac{1}{1 + \frac{1}{x}}$$

$$= 1$$